Micro_Rust_Parser_Experiment/Parser_Test_Flags.thy
@@ -1,0 +1,686 @@
+theory Parser_Test_Flags
+  imports Parser_Test_Utils
+begin
+
+section\<open> Default settings \<close>
+
+ML_val\<open>
+  local
+    val captured = Synchronized.var "urust_default_options" ([]: string list)
+    fun capture chunks = Synchronized.change captured (append chunks)
+    val _ =
+      Unsynchronized.setmp Private_Output.writeln_fn capture
+        (Attrib.print_options false) \<^context>
+    val output =
+      XML.content_of
+        (YXML.parse_body (implode (Synchronized.value captured)))
+    fun assert_default name =
+      if String.isSubstring (name ^ ": bool = false") output then ()
+      else
+        error
+          ("default value for " ^ quote name ^
+            " is not false in:\n" ^ output)
+    val _ =
+      List.app assert_default
+        ["urust_conformance_check", "urust_verbose", "urust_abbrev"]
+  in
+    val _ = ()
+  end
+\<close>
+
+urust_expr default_expr_flags \<open> () \<close>
+
+urust_fun default_fun_flags ::
+  \<open>(unit, unit, unit, unit, unit) function_body\<close>
+  ()
+  \<open> () \<close>
+
+
+section\<open> Inline flag combinations \<close>
+
+text\<open>
+Each command form exercises all eight Boolean combinations. The option order is deliberately varied.
+\<close>
+
+urust_expr
+  [urust_conformance_check = false, urust_verbose = false, urust_abbrev = false]
+  inline_expr_000 \<open> () \<close>
+urust_expr
+  [urust_abbrev = true, urust_conformance_check = false, urust_verbose = false]
+  inline_expr_001 \<open> () \<close>
+urust_expr
+  [urust_verbose = true, urust_abbrev = false, urust_conformance_check = false]
+  inline_expr_010 \<open> () \<close>
+urust_expr
+  [urust_conformance_check = false, urust_abbrev = true, urust_verbose = true]
+  inline_expr_011 \<open> () \<close>
+urust_expr
+  [urust_verbose = false, urust_conformance_check = true, urust_abbrev = false]
+  inline_expr_100 \<open> () \<close>
+urust_expr
+  [urust_abbrev = true, urust_verbose = false, urust_conformance_check = true]
+  inline_expr_101 \<open> () \<close>
+urust_expr
+  [urust_conformance_check = true, urust_verbose = true, urust_abbrev = false]
+  inline_expr_110 \<open> () \<close>
+urust_expr
+  [urust_verbose = true, urust_abbrev = true, urust_conformance_check = true]
+  inline_expr_111 \<open> () \<close>
+
+urust_fun
+  [urust_abbrev = false, urust_verbose = false, urust_conformance_check = false]
+  inline_fun_000 ::
+  \<open>(unit, unit, unit, unit, unit) function_body\<close> () \<open> () \<close>
+urust_fun
+  [urust_conformance_check = false, urust_abbrev = true, urust_verbose = false]
+  inline_fun_001 ::
+  \<open>(unit, unit, unit, unit, unit) function_body\<close> () \<open> () \<close>
+urust_fun
+  [urust_verbose = true, urust_conformance_check = false, urust_abbrev = false]
+  inline_fun_010 ::
+  \<open>(unit, unit, unit, unit, unit) function_body\<close> () \<open> () \<close>
+urust_fun
+  [urust_abbrev = true, urust_verbose = true, urust_conformance_check = false]
+  inline_fun_011 ::
+  \<open>(unit, unit, unit, unit, unit) function_body\<close> () \<open> () \<close>
+urust_fun
+  [urust_conformance_check = true, urust_abbrev = false, urust_verbose = false]
+  inline_fun_100 ::
+  \<open>(unit, unit, unit, unit, unit) function_body\<close> () \<open> () \<close>
+urust_fun
+  [urust_verbose = false, urust_conformance_check = true, urust_abbrev = true]
+  inline_fun_101 ::
+  \<open>(unit, unit, unit, unit, unit) function_body\<close> () \<open> () \<close>
+urust_fun
+  [urust_abbrev = false, urust_conformance_check = true, urust_verbose = true]
+  inline_fun_110 ::
+  \<open>(unit, unit, unit, unit, unit) function_body\<close> () \<open> () \<close>
+urust_fun
+  [urust_verbose = true, urust_conformance_check = true, urust_abbrev = true]
+  inline_fun_111 ::
+  \<open>(unit, unit, unit, unit, unit) function_body\<close> () \<open> () \<close>
+
+
+section\<open> Scoped settings and overrides \<close>
+
+declare [[urust_conformance_check = true]]
+declare [[urust_verbose = true]]
+declare [[urust_abbrev = true]]
+
+urust_expr scoped_all_true_expr \<open> () \<close>
+
+urust_fun scoped_all_true_fun ::
+  \<open>(unit, unit, unit, unit, unit) function_body\<close>
+  ()
+  \<open> () \<close>
+
+urust_expr
+  [urust_verbose = false, urust_abbrev = false, urust_conformance_check = false]
+  scoped_all_false_expr \<open> () \<close>
+
+urust_fun
+  [urust_conformance_check = false, urust_verbose = false, urust_abbrev = false]
+  scoped_all_false_fun ::
+  \<open>(unit, unit, unit, unit, unit) function_body\<close>
+  ()
+  \<open> () \<close>
+
+urust_expr [urust_abbrev = false]
+  scoped_partial_definition_expr \<open> () \<close>
+
+urust_fun [urust_conformance_check = false]
+  scoped_partial_abbrev_fun ::
+  \<open>(unit, unit, unit, unit, unit) function_body\<close>
+  ()
+  \<open> () \<close>
+
+declare [[urust_conformance_check = false]]
+declare [[urust_verbose = false]]
+declare [[urust_abbrev = false]]
+
+urust_expr reset_expr_flags \<open> () \<close>
+
+urust_fun reset_fun_flags ::
+  \<open>(unit, unit, unit, unit, unit) function_body\<close>
+  ()
+  \<open> () \<close>
+
+
+section\<open> Contextual expressions \<close>
+
+urust_expr [urust_conformance_check = true]
+  contextual_order
+  \<open> \<llangle>(first :: nat, second :: bool)\<rrangle> \<close>
+  with_args first second
+
+urust_expr [urust_conformance_check = true]
+  contextual_antiquotation
+  \<open> \<llangle>(left :: nat) + right\<rrangle> \<close>
+  with_args left right
+
+urust_expr [urust_conformance_check = true]
+  contextual_shadowing
+  \<open> let item = true; \<llangle>(item, outer :: nat)\<rrangle> \<close>
+  with_args item outer
+
+urust_expr
+  [urust_abbrev = true, urust_conformance_check = true, urust_verbose = true]
+  nie_contextual_helper
+  \<open> \<llangle>(address :: nat) + size\<rrangle> \<close>
+  with_args address size
+
+urust_expr contextual_definition_against
+  \<open> operand + 1u32 \<close>
+  with_args operand
+  against \<open> \<lbrakk> operand + 1_u32 \<rbrakk> \<close>
+
+urust_expr [urust_abbrev = true]
+  contextual_abbrev_against
+  \<open> operand + 2u32 \<close>
+  with_args operand
+  against \<open> \<lbrakk> operand + 2_u32 \<rbrakk> \<close>
+
+urust_fun fun_definition_against ::
+  \<open>32 word \<Rightarrow> (unit, 32 word, unit, unit, unit) function_body\<close>
+  (operand)
+  \<open> operand + 3u32 \<close>
+  against \<open> \<lbrakk> operand + 3_u32 \<rbrakk> \<close>
+
+urust_fun [urust_abbrev = true]
+  fun_abbrev_against ::
+  \<open>32 word \<Rightarrow> (unit, 32 word, unit, unit, unit) function_body\<close>
+  (operand)
+  \<open> operand + 4u32 \<close>
+  against \<open> \<lbrakk> operand + 4_u32 \<rbrakk> \<close>
+
+locale contextual_flags_locale =
+  fixes offset :: nat
+begin
+
+urust_expr [urust_abbrev = true, urust_conformance_check = true]
+  contextual_locale_helper
+  \<open> \<llangle>operand + offset\<rrangle> \<close>
+  with_args operand
+
+end
+
+ML_val\<open>
+  local
+    val ctxt = \<^context>
+    val first_pos =
+      Position.make0 11 100 0 "" "contextual-order-audit" ""
+    val second_pos =
+      Position.make0 11 110 0 "" "contextual-order-audit" ""
+    val source =
+      Parser_Lex_Util.positioned_content_source
+        "\<llangle>(first :: nat, second :: bool)\<rrangle>"
+        (Position.make0 13 200 0 "" "contextual-order-audit" "")
+    val actual =
+      URust_Command.elab_urust_with_args ctxt
+        [("first", first_pos), ("second", second_pos)] source
+    val expected =
+      Syntax.check_term ctxt
+        (Syntax.parse_term ctxt
+          "(\<lambda>(first :: nat) (second :: bool). \
+          \\<lbrakk> \<llangle>(first, second)\<rrangle> \<rbrakk>)")
+    val (formals, _) = Term.strip_abs actual
+    val function_body_count =
+      Term.fold_aterms
+        (fn Const (name, _) =>
+              if name = \<^const_name>\<open>FunctionBody\<close>
+              then Integer.add 1
+              else I
+          | _ => I)
+        actual 0
+    val _ =
+      if map #2 formals = [HOLogic.natT, HOLogic.boolT] then ()
+      else error "with_args: inferred argument types or source order changed"
+    val _ =
+      if Term.aconv (actual, expected) then ()
+      else error "with_args: contextual abstraction shape changed"
+    val _ =
+      if function_body_count = 0 then ()
+      else error "with_args: contextual expression gained a FunctionBody wrapper"
+  in
+    val _ = ()
+  end
+\<close>
+
+
+section\<open> Declaration artifacts \<close>
+
+definition expr_abbrev_client where
+  \<open> expr_abbrev_client = inline_expr_001 \<close>
+
+definition fun_abbrev_client where
+  \<open> fun_abbrev_client = inline_fun_001 \<close>
+
+ML_val\<open>
+  local
+    val ctxt = \<^context>
+    val thy = Proof_Context.theory_of ctxt
+    val consts = Proof_Context.consts_of ctxt
+
+    fun assert message condition =
+      if condition then () else error ("uRust flag artifact audit: " ^ message)
+
+    fun has_fact name = can (Proof_Context.get_thm ctxt) name
+
+    fun constant_name name =
+      Consts.intern consts name
+
+    fun is_abbreviation name =
+      can (Consts.the_abbreviation consts) (constant_name name)
+
+    fun executable_equations name =
+      let
+        val constant = constant_name name
+      in
+        (case Exn.result (Code.get_cert ctxt []) constant of
+           Exn.Res certificate =>
+             let
+               val (_, equations) =
+                 Code.equations_of_cert thy certificate
+             in
+               map_filter
+                 (fn (_, (SOME theorem, _)) => SOME theorem
+                   | _ => NONE)
+                 (the equations)
+             end
+         | Exn.Exn exn =>
+             if Exn.is_interrupt exn then Exn.reraise exn else [])
+      end
+
+    val definitions =
+      ["default_expr_flags", "default_fun_flags",
+       "inline_expr_000", "inline_expr_010",
+       "inline_expr_100", "inline_expr_110",
+       "inline_fun_000", "inline_fun_010",
+       "inline_fun_100", "inline_fun_110",
+       "scoped_all_false_expr", "scoped_all_false_fun",
+       "scoped_partial_definition_expr",
+       "reset_expr_flags", "reset_fun_flags",
+       "contextual_order", "contextual_antiquotation",
+       "contextual_shadowing", "contextual_definition_against",
+       "fun_definition_against"]
+
+    val abbreviations =
+      ["inline_expr_001", "inline_expr_011",
+       "inline_expr_101", "inline_expr_111",
+       "inline_fun_001", "inline_fun_011",
+       "inline_fun_101", "inline_fun_111",
+       "scoped_all_true_expr", "scoped_all_true_fun",
+       "scoped_partial_abbrev_fun", "nie_contextual_helper",
+       "contextual_abbrev_against", "fun_abbrev_against"]
+
+    val conforming =
+      ["inline_expr_100", "inline_expr_101",
+       "inline_expr_110", "inline_expr_111",
+       "inline_fun_100", "inline_fun_101",
+       "inline_fun_110", "inline_fun_111",
+       "scoped_all_true_expr", "scoped_all_true_fun",
+       "scoped_partial_definition_expr",
+       "contextual_order", "contextual_antiquotation",
+       "contextual_shadowing", "nie_contextual_helper",
+       "contextual_definition_against", "contextual_abbrev_against",
+       "fun_definition_against", "fun_abbrev_against"]
+
+    val nonconforming =
+      ["default_expr_flags", "default_fun_flags",
+       "inline_expr_000", "inline_expr_001",
+       "inline_expr_010", "inline_expr_011",
+       "inline_fun_000", "inline_fun_001",
+       "inline_fun_010", "inline_fun_011",
+       "scoped_all_false_expr", "scoped_all_false_fun",
+       "scoped_partial_abbrev_fun",
+       "reset_expr_flags", "reset_fun_flags"]
+
+    fun check_definition name =
+      (assert (quote name ^ " is missing its _def fact")
+         (has_fact (name ^ "_def"));
+       assert (quote name ^ " was registered as an abbreviation")
+         (not (is_abbreviation name));
+       assert (quote name ^ " does not have one code equation")
+         (length (executable_equations name) = 1))
+
+    fun check_abbreviation name =
+      (assert (quote name ^ " unexpectedly has a _def fact")
+         (not (has_fact (name ^ "_def")));
+       assert (quote name ^ " is not registered as an abbreviation")
+         (is_abbreviation name);
+       assert (quote name ^ " unexpectedly has a code equation")
+         (null (executable_equations name)))
+
+    val _ = List.app check_definition definitions
+    val _ = List.app check_abbreviation abbreviations
+    val _ =
+      List.app
+        (fn name =>
+          assert (quote name ^ " is missing _conformance")
+            (has_fact (name ^ "_conformance")))
+        conforming
+    val _ =
+      List.app
+        (fn name =>
+          assert (quote name ^ " unexpectedly has _conformance")
+            (not (has_fact (name ^ "_conformance"))))
+        nonconforming
+
+    fun assert_expanded client abbreviation =
+      let
+        val proposition =
+          Thm.prop_of (Proof_Context.get_thm ctxt (client ^ "_def"))
+        val abbreviation_name = constant_name abbreviation
+      in
+        assert
+          (quote abbreviation ^ " survived in checked client term")
+          (not
+            (Term.exists_subterm
+              (fn Const (name, _) => name = abbreviation_name
+                | _ => false)
+              proposition))
+      end
+
+    val _ = assert_expanded "expr_abbrev_client" "inline_expr_001"
+    val _ = assert_expanded "fun_abbrev_client" "inline_fun_001"
+  in
+    val _ = ()
+  end
+\<close>
+
+
+section\<open> Invalid flags and argument lists \<close>
+
+ML_val\<open>
+  local
+    val unit_source = Symbol.open_ ^ " () " ^ Symbol.close
+    val body_type =
+      Symbol.open_ ^
+      "(unit, unit, unit, unit, unit) function_body" ^
+      Symbol.close
+    val serial = Unsynchronized.ref 0
+
+    fun run_command source_name command_text () =
+      let
+        val thy = \<^theory>
+        val transitions =
+          Outer_Syntax.parse_text thy (K thy)
+            (Position.line_file 1 source_name) command_text
+        val _ =
+          if length transitions = 1 then ()
+          else error "expected exactly one parsed uRust command"
+      in
+        fold (Toplevel.command_exception false) transitions
+          (Toplevel.make_state (SOME thy))
+      end
+
+    fun recovery () =
+      let
+        val index = !serial
+        val _ = serial := index + 1
+      in
+        ignore
+          (run_command ("flag-recovery-" ^ string_of_int index)
+            ("urust_expr [urust_abbrev = true] recovered_" ^
+              string_of_int index ^ " " ^ unit_source) ())
+      end
+
+    fun assert_rejected source_name command_text expected =
+      (case Exn.result (run_command source_name command_text) () of
+         Exn.Res _ =>
+           error
+             ("invalid uRust command was unexpectedly accepted" ^
+               Position.here (Position.file source_name))
+       | Exn.Exn exn =>
+           if Exn.is_interrupt exn then Exn.reraise exn
+           else
+             let
+               val message = Runtime.exn_message exn
+               val _ =
+                 if String.isSubstring expected message andalso
+                    String.isSubstring source_name message
+                 then ()
+                 else
+                   error
+                     ("unexpected uRust command diagnostic:\n" ^ message ^
+                       "\nexpected: " ^ quote expected)
+             in recovery () end)
+
+    datatype command_kind = Expr | Fun
+
+    fun command Expr options name suffix =
+          "urust_expr " ^ options ^ " " ^ name ^ " " ^
+            unit_source ^ suffix
+      | command Fun options name suffix =
+          "urust_fun " ^ options ^ " " ^ name ^ " :: " ^
+            body_type ^ " () " ^ unit_source ^ suffix
+
+    fun mode_option false = "urust_abbrev = false"
+      | mode_option true = "urust_abbrev = true"
+
+    val kinds = [Expr, Fun]
+    val modes = [false, true]
+
+    fun test_unknown kind abbreviation =
+      let
+        val label =
+          "unknown-option-" ^
+          (case kind of Expr => "expr" | Fun => "fun") ^
+          (if abbreviation then "-abbrev" else "-definition")
+        val options =
+          "[" ^ mode_option abbreviation ^
+          ", urust_future_flag = true]"
+      in
+        assert_rejected label
+          (command kind options "unknown_flag" "")
+          "unknown uRust command option \"urust_future_flag\""
+      end
+
+    fun test_legacy legacy kind abbreviation =
+      let
+        val label =
+          "legacy-" ^ legacy ^ "-" ^
+          (case kind of Expr => "expr" | Fun => "fun") ^
+          (if abbreviation then "-abbrev" else "-definition")
+        val options =
+          "[" ^ mode_option abbreviation ^ ", " ^ legacy ^ " = true]"
+      in
+        assert_rejected label
+          (command kind options "legacy_flag" "")
+          ("unknown uRust command option " ^ quote legacy)
+      end
+
+    fun test_duplicate flag kind abbreviation =
+      let
+        val label =
+          "duplicate-" ^ flag ^ "-" ^
+          (case kind of Expr => "expr" | Fun => "fun") ^
+          (if abbreviation then "-abbrev" else "-definition")
+        val value = Bool.toString abbreviation
+        val options =
+          if flag = "urust_abbrev" then
+            "[" ^ flag ^ " = " ^ value ^ ", " ^
+              flag ^ " = " ^ value ^ "]"
+          else
+            "[" ^ mode_option abbreviation ^ ", " ^
+              flag ^ " = true, " ^ flag ^ " = false]"
+      in
+        assert_rejected label
+          (command kind options "duplicate_flag" "")
+          ("duplicate uRust command option " ^ quote flag)
+      end
+
+    fun test_contradiction kind abbreviation =
+      let
+        val label =
+          "contradictory-" ^
+          (case kind of Expr => "expr" | Fun => "fun") ^
+          (if abbreviation then "-abbrev" else "-definition")
+        val options =
+          "[" ^ mode_option abbreviation ^
+          ", urust_conformance_check = false]"
+        val suffix =
+          " against " ^ Symbol.open_ ^ " \<lbrakk> () \<rbrakk> " ^ Symbol.close
+      in
+        assert_rejected label
+          (command kind options "contradictory_flag" suffix)
+          "[urust_conformance_check = false] cannot be combined with `against`"
+      end
+
+    val _ = List.app (fn kind => List.app (test_unknown kind) modes) kinds
+    val _ =
+      List.app
+        (fn legacy =>
+          List.app
+            (fn kind => List.app (test_legacy legacy kind) modes)
+            kinds)
+        ["conformance_check", "verbose", "abbrev"]
+    val _ =
+      List.app
+        (fn flag =>
+          List.app
+            (fn kind => List.app (test_duplicate flag kind) modes)
+            kinds)
+        ["urust_conformance_check", "urust_verbose", "urust_abbrev"]
+    val _ =
+      List.app
+        (fn kind => List.app (test_contradiction kind) modes)
+        kinds
+
+    val _ =
+      assert_rejected "empty-with-args"
+        ("urust_expr empty_args " ^ unit_source ^ " with_args")
+        "`with_args` requires at least one argument"
+    val _ =
+      assert_rejected "wildcard-with-args"
+        ("urust_expr wildcard_args " ^ unit_source ^ " with_args _")
+        "argument name `_` is not allowed"
+    val _ =
+      assert_rejected "duplicate-with-args"
+        ("urust_expr duplicate_args " ^ unit_source ^ " with_args item item")
+        "duplicate argument \"item\""
+    val _ =
+      assert_rejected "misplaced-with-args"
+        ("urust_expr misplaced_args " ^ unit_source ^
+          " against " ^ Symbol.open_ ^ " \<lbrakk> () \<rbrakk> " ^ Symbol.close ^
+          " with_args item")
+        "command expected"
+  in
+    val _ = ()
+  end
+\<close>
+
+
+section\<open> Contextual binder markup \<close>
+
+ML_val\<open>
+  local
+    val ctxt = \<^context>
+    val file = "urust-with-args-markup-audit"
+    val document_id = "urust-with-args-markup-audit"
+    val first_definition =
+      Position.make0 11 100 0 "" file document_id
+    val second_definition =
+      Position.make0 11 110 0 "" file document_id
+    val body_text =
+      "\<llangle>(first :: nat, second :: bool, first)\<rrangle>"
+    val body_start =
+      Position.make0 13 200 0 "" file document_id
+    val body_source =
+      Parser_Lex_Util.positioned_content_source body_text body_start
+    val captured =
+      Synchronized.var "urust_with_args_markup" ([]: string list)
+    fun capture_reports chunks =
+      Synchronized.change captured (append chunks)
+
+    val _ =
+      Parser_Test_Report_Lock.run (fn () =>
+        Unsynchronized.setmp Private_Output.report_fn capture_reports
+          (fn () =>
+            Print_Mode.with_modes [Print_Mode.PIDE]
+              (fn () =>
+                URust_Command.elab_urust_with_args ctxt
+                  [("first", first_definition),
+                   ("second", second_definition)]
+                  body_source) ())
+          ())
+
+    fun collect (XML.Text _) result = result
+      | collect (XML.Elem (markup, body)) result =
+          fold collect body (markup :: result)
+    val markup =
+      fold collect
+        (maps YXML.parse_body (Synchronized.value captured)) []
+
+    fun find_from needle offset =
+      if offset + size needle > size body_text then
+        error ("with_args markup audit: missing " ^ quote needle)
+      else if String.substring (body_text, offset, size needle) = needle then
+        offset
+      else find_from needle (offset + 1)
+
+    fun token_position needle offset =
+      let
+        val raw = find_from needle offset
+        val start =
+          Position.symbol_explode
+            (String.substring (body_text, 0, raw)) body_start
+      in
+        (raw,
+         Position.range_position
+           (Position.range (start, Position.symbol_explode needle start)))
+      end
+
+    fun has_position properties position =
+      Properties.get properties Markup.offsetN =
+        Option.map Value.print_int (Position.offset_of position) andalso
+      Properties.get properties Markup.end_offsetN =
+        Option.map Value.print_int (Position.end_offset_of position)
+
+    fun entity_id property position =
+      let
+        val ids =
+          markup
+          |> map_filter
+              (fn (name, properties) =>
+                if name = Markup.entityN andalso
+                   Properties.get properties Markup.kindN =
+                     SOME "urust_var" andalso
+                   has_position properties position
+                then Properties.get properties property
+                else NONE)
+          |> distinct (op =)
+      in
+        (case ids of
+           [id] => id
+         | _ =>
+             error
+               ("with_args markup audit: binder entity markup changed at" ^
+                 Position.here position))
+      end
+
+    val (first_offset, first_reference_one) =
+      token_position "first" 0
+    val (second_offset, second_reference) =
+      token_position "second" (first_offset + size "first")
+    val (_, first_reference_two) =
+      token_position "first" (second_offset + size "second")
+    val first_id = entity_id Markup.defN first_definition
+    val second_id = entity_id Markup.defN second_definition
+    val _ =
+      if first_id <> second_id then ()
+      else error "with_args markup audit: arguments reused an entity ID"
+    val _ =
+      if entity_id Markup.refN first_reference_one = first_id andalso
+         entity_id Markup.refN first_reference_two = first_id
+      then ()
+      else error "with_args markup audit: first references lost navigation"
+    val _ =
+      if entity_id Markup.refN second_reference = second_id then ()
+      else error "with_args markup audit: second reference lost navigation"
+  in
+    val _ = ()
+  end
+\<close>
+
+end
